

DDA3020 Machine Learning

Gradient of Softmax Regression

10/14/2022

Recall the objective function of softmax regression:

$$\begin{aligned}
 J(\mathbf{W}) &= -\frac{1}{m} \sum_i^m \sum_j^C [\mathbb{I}(y_i = j) \log(f_{\mathbf{w}_j, b_j}(\mathbf{x}_i))] \\
 &= -\frac{1}{m} \sum_i^m \sum_j^C [\mathbb{I}(y_i = j) \log \frac{\exp(\mathbf{w}_j^\top \mathbf{x} + b_j)}{\sum_{c=1}^C \exp(\mathbf{w}_c^\top \mathbf{x} + b_c)}]
 \end{aligned} \tag{1}$$

Let $z_j = \mathbf{w}_j^\top \mathbf{x}_i + b_j$ and $f_j = f_{\mathbf{w}_j, b_j}(\mathbf{x}_i) = \frac{\exp(z_j)}{\sum_{c=1}^C \exp(z_c)}$. Consider one sample for convenience.

$$\begin{aligned}
 \frac{\partial J_i}{\partial z_k} &= -\sum_{j=1}^C \left[\mathbb{I}(y_i = j) \frac{1}{f_j} \frac{\partial f_j}{\partial z_k} \right] \\
 &= -\left(\sum_{j=k}^C \left[\mathbb{I}(y_i = j) \frac{1}{f_j} \frac{\partial f_j}{\partial z_k} \right] + \sum_{j \neq k}^C \left[\mathbb{I}(y_i = j) \frac{1}{f_j} \frac{\partial f_j}{\partial z_k} \right] \right) \\
 &= -\left(\left[\mathbb{I}(y_i = k) \frac{1}{f_k} \frac{\partial f_k}{\partial z_k} \right] + \sum_{j \neq k}^C \left[\mathbb{I}(y_i = j) \frac{1}{f_j} \frac{\partial f_j}{\partial z_k} \right] \right) \\
 &= -\left[\mathbb{I}(y_i = k) \frac{1}{f_k} \left(\frac{\exp(z_k)}{\sum_{c=1}^C \exp(z_c)} - \frac{\exp(z_k) \exp(z_k)}{\left(\sum_{c=1}^C \exp(z_c) \right)^2} \right) \right] \\
 &\quad - \sum_{j \neq k}^C \left[-\mathbb{I}(y_i = j) \frac{1}{f_j} \frac{\exp(z_j) \exp(z_k)}{\left(\sum_{c=1}^C \exp(z_c) \right)^2} \right] \\
 &= -\left(\mathbb{I}(y_i = k) \frac{1}{f_k} \times (f_k - f_k^2) - \sum_{j \neq k}^C \mathbb{I}(y_i = j) \frac{1}{f_j} \times f_j \times f_k \right) \\
 &= -\left(\mathbb{I}(y_i = k) - \mathbb{I}(y_i = k) f_k - \sum_{j \neq k}^C \mathbb{I}(y_i = j) f_k \right) \\
 &= -\left(\mathbb{I}(y_i = k) - \sum_{j=1}^C \mathbb{I}(y_i = j) f_k \right) \quad \text{Note that } \sum_{j=1}^C \mathbb{I}(y_i = j) = 1 \\
 &= f_k - \mathbb{I}(y_i = k)
 \end{aligned} \tag{2}$$

Now we obtain

$$\frac{\partial J}{\partial \mathbf{w}_k} = \frac{1}{m} \sum_{i=1}^m \frac{\partial J_i}{\partial z_k} \frac{\partial z_k}{\partial \mathbf{w}_k} = \frac{1}{m} \sum_{i=1}^m (f_k - \mathbb{I}(y_i = k)) \mathbf{x}_i \tag{3}$$